Finished Step0 and Step1

ntor/Games.ec
@@ -21,19 +21,40 @@ import GAKEc.
     * if not => Gap-DH another way.
 *)
 
-(* Removing key collisions *)
-module Game1 = {
+(* Step0 inlining everything and adding bad event *)
+module Game0 : GAKE_out_i = {
   var servers : (s_id, server_state) fmap
 
   var c_smap : (int, pr_st_client instance_state) fmap
   var s_smap : (s_id * int, pr_st_server instance_state) fmap
   
-  var keypairs : ((pkey * skey)) fset
+  var kp_set : ((pkey * skey)) fset
+  var bad : bool
 
   proc init_mem() : unit = {
     servers <- empty;
     c_smap <- empty;
     s_smap <- empty;
+    kp_set <- fset0;
+    bad <- false;
+  }
+  
+  (* random oracle *)
+  proc h(input: pkey * pkey * s_id * pkey * pkey) : tag * key = {
+    return hash_ntor input.`1 input.`2 input.`3 input.`4 input.`5;
+  }
+
+  (* server management *)
+  proc init_s(b: s_id) : pkey option = {
+    var kp;
+
+    if (b \notin servers) {
+      kp <$ dkp;
+      bad <- bad \/ kp \in kp_set;
+      kp_set <- kp_set `|` fset1 kp;
+      servers.[b] <- Honest kp;
+    }
+    return omap get_pkey servers.[b];
   }
   
   proc set_cert(b: s_id, pk: pkey) : unit option = {
@@ -46,17 +67,6 @@ module Game1 = {
     return r;
   }
 
-
-  proc init_s(b: s_id) : pkey option = {
-    var kp;
-
-    if (b \notin servers) {
-      kp <$ dkp;
-      servers.[b] <- Honest kp;
-    }
-    return omap get_pkey servers.[b];
-  }
-
   proc send_msg1(i: int, m1: s_id) : pkey option = {
     var st, pk_b, kp;
     var r <- None;
@@ -67,12 +77,14 @@ module Game1 = {
       match st with
       | None => {
           kp <$ dkp;
+          bad <- bad \/ kp \in kp_set;
+          kp_set <- kp_set `|` fset1 kp;
           c_smap.[i] <- Pending (m1, pk_b, fst kp, snd kp) (fst kp) (false, false, false);
           r <- Some (fst kp);
         }
       | Some st => {
           match st with
-          | Pending st _ ir => c_smap.[i] <- Aborted (Some st) None ir;
+          | Pending st pt ir => c_smap.[i] <- Aborted (Some st) (Some (pt, None)) ir;
           | Accepted _ _ _ _ => { }
           | Aborted _ _ _ => { }
           end;
@@ -83,17 +95,19 @@ module Game1 = {
   }
 
   proc send_msg2(b: s_id, j: int, m2: pkey) : (pkey * tag) option = {
-    var sko, pk_se, sk_se, t_B, sk;
+    var sko, kp, t_B, sk;
     var r <- None;
 
     sko <- obind get_skey servers.[b];
     if (sko is Some sk_b) (* Server was initialised as honest *) {
       match s_smap.[b, j] with
       | None => {
-          (pk_se, sk_se) <$ dkp;
-          (t_B, sk) <- hash_ntor (m2 ^ sk_se) (m2 ^ sk_b) b m2 pk_se;
-          s_smap.[(b, j)] <- Accepted (b, sk_b, Some sk_se) (m2, Some (pk_se, t_B)) sk (false, false, false);
-          r <- Some (pk_se, t_B);
+          kp <$ dkp;
+          bad <- bad \/ kp \in kp_set;
+          kp_set <- kp_set `|` fset1 kp;
+          (t_B, sk) <- hash_ntor (m2 ^ kp.`2) (m2 ^ sk_b) b m2 kp.`1;
+          s_smap.[(b, j)] <- Accepted (b, sk_b, Some kp.`2) (m2, Some (kp.`1, t_B)) sk (false, false, false);
+          r <- Some (kp.`1, t_B);
         }
       | Some st => { (* only completed sessions would be stored, and those can't be aborted; do nothing *) }
       end;
@@ -128,15 +142,18 @@ module Game1 = {
     return r;
   }
 
-  (* reveal and test *)
+
+(* reveal and test *)
   proc c_rev_skey(i: int) : key option = {
     var k <- None;
 
     match c_smap.[i] with
     | None => { }
     | Some _ => {
+        (* only accepted client instances that are not tested and 
+           that not only have tested partners can be sesskey revealed *)
         if (oget c_smap.[i] is Accepted st' t' k' ir') {
-          if (!get_ir_test (oget c_smap.[i]) /\ untested_partner_c t' s_smap <> Some false) {
+          if (!(get_ir_test (oget c_smap.[i]) \/ untested_partner_c t' s_smap = Some false)) {
             k <- Some k';
             c_smap.[i] <- set_ir_sess (Accepted st' t' k' ir');
           }
@@ -152,8 +169,10 @@ module Game1 = {
     match s_smap.[(b, j)] with
     | None => { }
     | Some _ => {
+        (* only accepted server instances that are not tested and 
+           that not only have tested partners can be sesskey revealed *)
         if (oget s_smap.[b, j] is Accepted st' t' k' ir') {
-          if (!get_ir_test (oget s_smap.[b, j]) /\ untested_partner_s t' c_smap <> Some false) {
+          if (!(get_ir_test (oget s_smap.[b, j]) \/ untested_partner_s t' c_smap = Some false)) {
             k <- Some k';
             s_smap.[(b, j)] <- set_ir_sess (Accepted st' t' k' ir');
           }
@@ -169,9 +188,11 @@ module Game1 = {
     match servers.[b] with
     | None => { }
     | Some _ => {
+        (* a server can be ltkey revealed if no instance of it is ephkey revealed 
+           in case that instance or all its partners are tested *) 
         if (oget servers.[b] is Honest kp) {
           if (forall j,
-                (b, j) \in s_smap
+                (b, j) \in s_smap (* just checking instances of b *)
                 => !(   (   get_ir_test (oget s_smap.[b, j])
                             (* This is always OK (get_trace always Some on server side *)
                          \/ untested_partner_s (oget (get_trace (oget s_smap.[b, j]))) c_smap = Some false)
@@ -192,14 +213,18 @@ module Game1 = {
     | None => { }
     | Some _ => {
         match oget c_smap.[i] with
+          (* client instances can be ephkey revealed when pending if there isn't 
+             a tested origin partner (agreeing on first message *)
         | Pending st pk_e ir => {
-            if (untested_partner_c (pk_e, None) s_smap <> Some false) {
+            if (untested_origins_c (pk_e, None) s_smap <> Some false) {
               ek <- Some (get_eph_c st);
               c_smap.[i] <- set_ir_eph (Pending st pk_e ir);
             }
           }
+          (* accepted client instamces can only be ephkey revealed when not tested and 
+             if not all partners are tested *)
         | Accepted st t k ir => {
-            if (!get_ir_test (oget c_smap.[i]) /\ untested_partner_c t s_smap <> Some false) {
+            if (!(get_ir_test (oget c_smap.[i]) \/ untested_partner_c t s_smap = Some false)) {
               ek <- Some (get_eph_c st);
               c_smap.[i] <- set_ir_eph (Accepted st t k ir);
             }
@@ -217,6 +242,8 @@ module Game1 = {
     match s_smap.[b, j] with
     | None => { }
     | Some _ => {
+        (* only accepted server instances that are not ltkey revealed in case they 
+           or all partners are tested can be ephkey revealed *)
         if (oget s_smap.[b, j] is Accepted st t k ir) { (* No Pending on Server side *)
           if (!((   get_ir_test (oget s_smap.[b, j])
                  \/ untested_partner_s t c_smap = Some false)
@@ -236,9 +263,11 @@ module Game1 = {
     match c_smap.[i] with
     | None => { }
     | Some _ => {
+        (* only accepted client instances that are not sesskey revealed, not ephkey revealed 
+           and not all partner instances are unfresh can be tested *)
         if (oget c_smap.[i] is Accepted st' t' k' ir') {
-          if (   !get_ir_sess (oget c_smap.[i]) /\ !get_ir_eph (oget c_smap.[i]) 
-              /\ fresh_partner_c t' s_smap servers <> Some false) {
+          if (!(   get_ir_sess (oget c_smap.[i]) \/ get_ir_eph (oget c_smap.[i]) 
+                \/ fresh_partner_c t' s_smap servers = Some false)) {
             k <- Some k';
             c_smap.[i] <- set_ir_test (Accepted st' t' k' ir');
           }
@@ -254,10 +283,12 @@ module Game1 = {
     match s_smap.[(b, j)] with
     | None => { }
     | Some _ => {
+        (* only accepted server instances that are not sesskey revealed, not trivially broken
+           and not all partner instances are unfresh can be tested *)
         if (oget s_smap.[b, j] is Accepted st' t' k' ir') {
-          if (   !get_ir_sess (oget s_smap.[b, j]) 
-              /\ !(get_ir_eph (oget s_smap.[b, j]) /\ get_sr_ltk (oget servers.[b]))
-              /\ fresh_partner_s t' c_smap <> Some false) {
+          if (!(   get_ir_sess (oget s_smap.[b, j]) 
+                \/ (get_ir_eph (oget s_smap.[b, j]) /\ get_sr_ltk (oget servers.[b]))
+                \/ fresh_partner_s t' c_smap = Some false)) {
             k <- Some k';
             s_smap.[(b, j)] <- set_ir_test (Accepted st' t' k' ir');
           }
@@ -267,3 +298,23 @@ module Game1 = {
     return k;
   }
 }.
+
+print Game0.
+
+(* Step1: Removing key collisions *)
+module Game1 = Game0 with {
+  proc init_s [
+    ^if.^bad<- + (!bad)
+  ]
+
+  proc send_msg1 [
+    ^if.^match#None.^bad<- + (!bad)
+  ]
+
+  proc send_msg2 [
+    ^match#Some.^match#None.^bad<- + (!bad)
+  ]
+}.
+
+print Game1.
+
