ntor/Security.ec
@@ -11,6 +11,202 @@ import GAKEc.
 (* ------------------------------------------------------------------------------------------ *)
 section.
 
-declare module A <: A_GAKE {-GAKE0}.
+declare module A <: A_GAKE {-GAKE0, -Game0, -Game1}.
+
+declare axiom A_ll:
+forall (G <: GAKE_out{-A}),
+  islossless G.h =>
+  islossless G.init_s =>
+  islossless G.set_cert =>
+  islossless G.send_msg1 =>
+  islossless G.send_msg2 =>
+  islossless G.send_msg3 =>
+  islossless G.c_rev_skey =>
+  islossless G.s_rev_skey =>
+  islossless G.rev_ltkey =>
+  islossless G.c_rev_ephkey =>
+  islossless G.s_rev_ephkey =>
+  islossless G.c_test => islossless G.s_test => islossless A(G).run.
+
+
+lemma Step0 &m :
+  Pr[E_GAKE(GAKE0(NTOR_S, NTOR_C), A).run() @ &m : res] = Pr[E_GAKE(Game0, A).run() @ &m : res].
+proof. 
+byequiv => //.
+proc; inline*.
+sim (: ={servers, c_smap, s_smap}(GAKE0, Game0)).
+
+- proc; inline*; by auto => /#.
+
+- proc; inline*.
+  sp; match = => //.
+  move => sk.
+  match = => //.
+  match Some {1} 4.
+   + by auto; smt(mem_set).
+  match Some {1} 10.
+  + by auto; smt().
+  auto => />.
+
+- proc; inline*. 
+  sp; if => //.
+  sp; match = => //.
+  auto => />. 
+  move => st.
+  match = => //.
+  move => st' pt' ir'.
+  auto => />.
+
+- proc; inline*.
+  if => //.
+  auto => /#.
+qed.
+
+lemma Step1 &m: `| Pr[E_GAKE(Game0, A).run() @ &m : res] - Pr[E_GAKE(Game1, A).run() @ &m : res] | <= Pr[E_GAKE(Game1, A).run() @ &m : Game1.bad].
+proof.
+byequiv (: _ ==> _) : Game0.bad => //; first last.
++ move=> &1 &2.
+  by case: (Game1.bad{2}).
+proc; inline*.
+call (: Game1.bad, ={servers, c_smap, s_smap, kp_set, bad}(Game0, Game1), ={bad}(Game0, Game1)) => //. 
+
+- exact A_ll.
+
+- proc; auto => />.
+- move => &2 bad.
+  proc; auto => />. 
+- move => &1. 
+  proc; auto => />.
+
+- proc.
+  if => //.
+  seq 1 1: (#pre /\ ={kp}); 1: by auto.
+  by sp 0 1; if{2}; auto => />.
+- move => &2 bad.
+  proc; if; auto.
+  rewrite dkp_ll //=. smt().
+- move => &1. 
+  proc; if => //. 
+  rcondf ^if; auto => />.
+  by rewrite dkp_ll.
+
+- proc; auto => />.
+- move => &2 bad.
+  proc; auto => />.
+- move => &1. 
+  proc; auto => />. 
+
+- proc.
+  sp; if => //.
+  sp; match = => //. 
+  + seq 1 1: (#pre /\ ={kp}); 1: by auto.
+    by sp 0 1; if{2}; auto => />.
+  move => st. 
+  match = => //.
+  move => st' pr' ir'.
+  auto => />.
+- move => &2 bad.
+  proc; sp; if => //; sp. 
+  match; auto => />.
+  + rewrite dkp_ll. smt().
+  by smt().
+- move => &1. 
+  proc; sp; if => //. 
+  sp; match; auto => />.
+  + by rewrite dkp_ll.
+  by smt().
+
+- proc.
+  sp; match = => //. 
+  move => sk.
+  match = => //.
+  + seq 1 1: (#pre /\ ={kp}); 1: by auto.
+    by sp 0 1; if{2}; auto => />.
+- move => &2 bad.
+  proc; sp; match; auto => />.
+  match; auto => />.
+  rewrite dkp_ll. 
+  by smt().
+- move => &1. 
+  proc; sp; match; auto => />.
+  match; auto => />.
+  by rewrite dkp_ll.
+
+- proc; auto => />. 
+  by smt().
+- move => &2 bad.
+  proc; auto => />.
+  by smt().
+- move => &1.
+  proc; auto => />.
+  by smt().
+
+- proc; auto => />. 
+  by smt().
+- move => &2 bad.
+  proc; auto => />.
+  by smt().
+- move => &1.
+  proc; auto => />.
+  by smt().
+
+- proc; auto => />. 
+  by smt().
+- move => &2 bad.
+  proc; auto => />.
+  by smt().
+- move => &1.
+  proc; auto => />.
+  by smt().
+
+- proc; auto => />. 
+  by smt().
+- move => &2 bad.
+  proc; auto => />.
+  by smt().
+- move => &1.
+  proc; auto => />.
+  by smt().
+
+- proc; auto => />. 
+  by smt().
+- move => &2 bad.
+  proc; auto => />.
+  by smt().
+- move => &1.
+  proc; auto => />.
+  by smt().
+
+- proc; auto => />. 
+  by smt().
+- move => &2 bad.
+  proc; auto => />.
+  by smt().
+- move => &1.
+  proc; auto => />.
+  by smt().
+
+- proc; auto => />. 
+  by smt().
+- move => &2 bad.
+  proc; auto => />.
+  by smt().
+- move => &1.
+  proc; auto => />.
+  by smt().
+
+- proc; auto => />. 
+  by smt().
+- move => &2 bad.
+  proc; auto => />.
+  by smt().
+- move => &1.
+  proc; auto => />.
+  by smt().
+
+auto => />.
+move => rl rr al bl dl pl kpl sl ar br dr pr kpr sr. 
+by case : (!br) => />.
+qed.
 
 end section.
